MathematicalLogic/FirstOrder/Semantics.lean
@@ -4,25 +4,21 @@ universe u v
 
 namespace FirstOrder.Language
 
-structure Structure (𝓛 : Language) where
-  Dom : Type u
-  interpFunc : 𝓛.Func n → Vec Dom n → Dom
-  interpRel : 𝓛.Rel n → Vec Dom n → Prop
+class IsStructure (𝓛 : Language) (𝓜 : Type u) where
+  interpFunc : 𝓛.Func n → Vec 𝓜 n → 𝓜
+  interpRel : 𝓛.Rel n → Vec 𝓜 n → Prop
 
-variable {𝓛 : Language} {𝓜 : 𝓛.Structure}
+variable {𝓛 : Language} {𝓜 : Type u} [𝓛.IsStructure 𝓜] {t t₁ t₂ : 𝓛.Term n} {p q : 𝓛.Formula n}
 
-namespace Structure
+open IsStructure
 
-instance : CoeSort 𝓛.Structure (Type u) := ⟨(·.Dom)⟩
-
-abbrev Assignment (𝓜 : 𝓛.Structure) (n : ℕ) := Vec 𝓜 n
-
-def interp (𝓜 : 𝓛.Structure) : 𝓛.Term n → 𝓜.Assignment n → 𝓜
+def interp (𝓜 : Type u) [𝓛.IsStructure 𝓜] : 𝓛.Term n → Vec 𝓜 n → 𝓜
 | #x, ρ => ρ x
-| f ⬝ᶠ v, ρ => 𝓜.interpFunc f λ i => 𝓜.interp (v i) ρ
-notation:80 "⟦" t "⟧ₜ " 𝓜 ", " ρ:80 => interp 𝓜 t ρ
-@[simp] theorem interp_var : ⟦ #x ⟧ₜ 𝓜, ρ = ρ x := rfl
-@[simp] theorem interp_func : ⟦ f ⬝ᶠ v ⟧ₜ 𝓜, ρ = 𝓜.interpFunc f λ i => ⟦ v i ⟧ₜ 𝓜, ρ := rfl
+| f ⬝ᶠ v, ρ => interpFunc f λ i => interp 𝓜 (v i) ρ
+notation:80 "⟦" t "⟧ₜ " α ", " ρ:80 => interp α t ρ
+
+@[simp] theorem interp_var : ⟦ (#x : 𝓛.Term n) ⟧ₜ 𝓜, ρ = ρ x := rfl
+@[simp] theorem interp_func : ⟦ (f ⬝ᶠ v : 𝓛.Term n) ⟧ₜ 𝓜, ρ = interpFunc f λ i => ⟦ v i ⟧ₜ 𝓜, ρ := rfl
 
 theorem interp_subst : ⟦ t[σ]ₜ ⟧ₜ 𝓜, ρ = ⟦ t ⟧ₜ 𝓜, λ x => ⟦ σ x ⟧ₜ 𝓜, ρ := by
   induction t with simp
@@ -31,32 +27,34 @@ theorem interp_subst : ⟦ t[σ]ₜ ⟧ₜ 𝓜, ρ = ⟦ t ⟧ₜ 𝓜, λ x =>
 theorem interp_shift : ⟦ ↑ₜt ⟧ₜ 𝓜, (u ∷ᵥ ρ) = ⟦ t ⟧ₜ 𝓜, ρ := by
   simp [Term.shift, interp_subst]
 
-def satisfy (𝓜 : 𝓛.Structure) : {n : ℕ} → 𝓛.Formula n → 𝓜.Assignment n → Prop
-| _, r ⬝ʳ v, ρ => 𝓜.interpRel r λ i => ⟦ v i ⟧ₜ 𝓜, ρ
+def satisfy (𝓜 : Type u) [𝓛.IsStructure 𝓜] : {n : ℕ} → 𝓛.Formula n → Vec 𝓜 n → Prop
+| _, r ⬝ʳ v, ρ => interpRel r λ i => ⟦ v i ⟧ₜ 𝓜, ρ
 | _, t₁ ≐ t₂, ρ => ⟦ t₁ ⟧ₜ 𝓜, ρ = ⟦ t₂ ⟧ₜ 𝓜, ρ
 | _, ⊥, _ => False
-| _, p ⇒ q, ρ => 𝓜.satisfy p ρ → 𝓜.satisfy q ρ
-| _, ∀' p, ρ => ∀ u, 𝓜.satisfy p (u ∷ᵥ ρ)
+| _, p ⇒ q, ρ => satisfy 𝓜 p ρ → satisfy 𝓜 q ρ
+| _, ∀' p, ρ => ∀ u, satisfy 𝓜 p (u ∷ᵥ ρ)
 notation:50 𝓜 " ⊨[" ρ "] " p:50 => satisfy 𝓜 p ρ
-@[simp] theorem satisfy_rel : 𝓜 ⊨[ρ] r ⬝ʳ v ↔ 𝓜.interpRel r λ i => ⟦ v i ⟧ₜ 𝓜, ρ := by rfl
+
+@[simp] theorem satisfy_rel : 𝓜 ⊨[ρ] (r ⬝ʳ v : 𝓛.Formula n) ↔ interpRel r λ i => ⟦ v i ⟧ₜ 𝓜, ρ := by rfl
 @[simp] theorem satisfy_eq : 𝓜 ⊨[ρ] t₁ ≐ t₂ ↔ ⟦ t₁ ⟧ₜ 𝓜, ρ = ⟦ t₂ ⟧ₜ 𝓜, ρ := by rfl
-@[simp] theorem satisfy_false : ¬ 𝓜 ⊨[ρ] ⊥ := by tauto
+@[simp] theorem satisfy_false : ¬ 𝓜 ⊨[ρ] (⊥ : 𝓛.Formula n) := by tauto
 @[simp] theorem satisfy_imp : 𝓜 ⊨[ρ] p ⇒ q ↔ 𝓜 ⊨[ρ] p → 𝓜 ⊨[ρ] q := by rfl
-@[simp] theorem satisfy_true : 𝓜 ⊨[ρ] ⊤ := by tauto
+@[simp] theorem satisfy_true : 𝓜 ⊨[ρ] (⊤ : 𝓛.Formula n) := by tauto
 @[simp] theorem satisfy_neg : 𝓜 ⊨[ρ] ~ p ↔ ¬ 𝓜 ⊨[ρ] p := by rfl
 @[simp] theorem satisfy_and : 𝓜 ⊨[ρ] p ⩑ q ↔ 𝓜 ⊨[ρ] p ∧ 𝓜 ⊨[ρ] q := by simp [PropNotation.and]
 @[simp] theorem satisfy_or : 𝓜 ⊨[ρ] p ⩒ q ↔ 𝓜 ⊨[ρ] p ∨ 𝓜 ⊨[ρ] q := by simp [PropNotation.or]; tauto
 @[simp] theorem satisfy_iff : 𝓜 ⊨[ρ] p ⇔ q ↔ (𝓜 ⊨[ρ] p ↔ 𝓜 ⊨[ρ] q) := by simp [PropNotation.iff]; tauto
-@[simp] theorem satisfy_all : 𝓜 ⊨[ρ] ∀' p ↔ ∀ u, 𝓜 ⊨[u ∷ᵥ ρ] p := by rfl
-@[simp] theorem satisfy_ex : 𝓜 ⊨[ρ] ∃' p ↔ ∃ u, 𝓜 ⊨[u ∷ᵥ ρ] p := by simp [Formula.ex]
+@[simp] theorem satisfy_all {p : 𝓛.Formula (n + 1)} : 𝓜 ⊨[ρ] ∀' p ↔ ∀ u, 𝓜 ⊨[u ∷ᵥ ρ] p := by rfl
+@[simp] theorem satisfy_ex {p : 𝓛.Formula (n + 1)} : 𝓜 ⊨[ρ] ∃' p ↔ ∃ u, 𝓜 ⊨[u ∷ᵥ ρ] p := by simp [Formula.ex]
 
 theorem satisfy_andN {v : Vec (𝓛.Formula n) m} :
   𝓜 ⊨[ρ] (⋀ i, v i) ↔ ∀ i, 𝓜 ⊨[ρ] v i := by
   induction m with simp [Formula.andN]
   | succ n ih => simp [Vec.head, ih, Fin.forall_fin_succ]
 
-theorem satisfy_subst {σ : 𝓛.Subst m n} : 𝓜 ⊨[ρ] p[σ]ₚ ↔ 𝓜 ⊨[λ x => ⟦ σ x ⟧ₜ 𝓜, ρ] p := by
-  induction p generalizing n with simp
+theorem satisfy_subst {σ : 𝓛.Subst n m} :
+  𝓜 ⊨[ρ] p[σ]ₚ ↔ 𝓜 ⊨[λ x => ⟦ σ x ⟧ₜ 𝓜, ρ] p := by
+  induction p generalizing m with simp
   | rel | eq => simp [interp_subst]
   | imp p q ih₁ ih₂ => simp [ih₁, ih₂]
   | all p ih =>
@@ -65,12 +63,14 @@ theorem satisfy_subst {σ : 𝓛.Subst m n} : 𝓜 ⊨[ρ] p[σ]ₚ ↔ 𝓜 ⊨
     congr! with x
     cases x using Fin.cases <;> simp [interp_shift]
 
-theorem satisfy_subst_single : 𝓜 ⊨[ρ] p[↦ₛ t]ₚ ↔ 𝓜 ⊨[ ⟦t⟧ₜ 𝓜, ρ ∷ᵥ ρ ] p := by
+theorem satisfy_subst_single {p : 𝓛.Formula (n + 1)} :
+  𝓜 ⊨[ρ] p[↦ₛ t]ₚ ↔ 𝓜 ⊨[ ⟦t⟧ₜ 𝓜, ρ ∷ᵥ ρ ] p := by
   simp [satisfy_subst]
   congr! with x
   cases x using Fin.cases <;> simp
 
-theorem satisfy_subst_assign : 𝓜 ⊨[ρ] p[≔ₛ t]ₚ ↔ 𝓜 ⊨[ ⟦t⟧ₜ 𝓜, ρ ∷ᵥ ρ.tail ] p := by
+theorem satisfy_subst_assign {p : 𝓛.Formula (n + 1)} {t} :
+  𝓜 ⊨[ρ] p[≔ₛ t]ₚ ↔ 𝓜 ⊨[ ⟦t⟧ₜ 𝓜, ρ ∷ᵥ ρ.tail ] p := by
   simp [satisfy_subst]
   congr! with x
   cases x using Fin.cases <;> simp
@@ -78,10 +78,10 @@ theorem satisfy_subst_assign : 𝓜 ⊨[ρ] p[≔ₛ t]ₚ ↔ 𝓜 ⊨[ ⟦t⟧
 theorem satisfy_shift : 𝓜 ⊨[u ∷ᵥ ρ] ↑ₚp ↔ 𝓜 ⊨[ρ] p := by
   simp [Formula.shift, satisfy_subst]
 
-abbrev satisfySentence (𝓜 : 𝓛.Structure) (p : 𝓛.Sentence) := 𝓜 ⊨[[]ᵥ] p
+abbrev satisfySentence (𝓜 : Type u) [𝓛.IsStructure 𝓜] (p : 𝓛.Sentence) := 𝓜 ⊨[[]ᵥ] p
 infix:50 " ⊨ₛ " => satisfySentence
 
-theorem satisfy_alls {p : 𝓛.Formula n} : 𝓜 ⊨ₛ ∀* p ↔ ∀ ρ, 𝓜 ⊨[ρ] p := by
+theorem satisfy_alls : 𝓜 ⊨ₛ ∀* p ↔ ∀ ρ, 𝓜 ⊨[ρ] p := by
   induction n with simp [Formula.alls]
   | zero => rfl
   | succ n ih =>
@@ -90,12 +90,23 @@ theorem satisfy_alls {p : 𝓛.Formula n} : 𝓜 ⊨ₛ ∀* p ↔ ∀ ρ, 𝓜 
     · intro h ρ; rw [Vec.eq_cons ρ]; apply h
     · intro h ρ u; exact h (u ∷ᵥ ρ)
 
+structure Structure (𝓛 : Language) where
+  Dom : Type u
+  interpFunc {n} : 𝓛.Func n → Vec Dom n → Dom
+  interpRel {n} : 𝓛.Rel n → Vec Dom n → Prop
+
+namespace Structure
+
+instance : CoeSort 𝓛.Structure (Type u) := ⟨(·.Dom)⟩
+instance {𝓜 : 𝓛.Structure} : 𝓛.IsStructure 𝓜 := ⟨𝓜.interpFunc, 𝓜.interpRel⟩
+@[reducible] def of (𝓜 : Type u) [𝓛.IsStructure 𝓜] : 𝓛.Structure := ⟨𝓜, IsStructure.interpFunc, IsStructure.interpRel⟩
+
 end Structure
 
 
 
-def Entails (Γ : 𝓛.FormulaSet n) (p) :=
-  ∀ (𝓢 : Structure.{u} 𝓛) (ρ), (∀ q ∈ Γ, 𝓢 ⊨[ρ] q) → 𝓢 ⊨[ρ] p
+def Entails (Γ : 𝓛.FormulaSet n) (p : 𝓛.Formula n) :=
+  ∀ (𝓜 : Structure.{u} 𝓛) (ρ), (∀ q ∈ Γ, 𝓜 ⊨[ρ] q) → 𝓜 ⊨[ρ] p
 
 infix:50 " ⊨ " => Entails
 syntax:50 term " ⊨.{" level "} " term:50 : term
@@ -116,41 +127,45 @@ theorem Satisfiable.weaken :
 
 namespace Theory
 
+class IsModel (𝓣 : 𝓛.Theory) (𝓜 : Type u) [𝓛.IsStructure 𝓜] : Prop where
+  satisfy_theory : ∀ p ∈ 𝓣, 𝓜 ⊨ₛ p
+
 structure Model (𝓣 : 𝓛.Theory) extends 𝓛.Structure where
   satisfy_theory : ∀ p ∈ 𝓣, toStructure ⊨ₛ p
 
-variable {𝓣 : 𝓛.Theory}
+variable {𝓣 : 𝓛.Theory} {𝓜 : 𝓣.Model} {p q : 𝓛.Sentence}
+
+namespace Model
 
 instance : CoeOut 𝓣.Model 𝓛.Structure := ⟨(·.toStructure)⟩
 instance : CoeSort 𝓣.Model (Type u) := ⟨(·.Dom)⟩
+instance : 𝓣.IsModel 𝓜 := ⟨𝓜.satisfy_theory⟩
 
-theorem entails_iff {𝓣 : 𝓛.Theory} : 𝓣 ⊨.{u} p ↔ ∀ (𝓜 : Model.{u} 𝓣), 𝓜 ⊨ₛ p := by
+def of (𝓜 : Type u) [𝓛.IsStructure 𝓜] [𝓣.IsModel 𝓜] : 𝓣.Model := ⟨Structure.of 𝓜, IsModel.satisfy_theory⟩
+
+end Model
+
+theorem entails_iff : 𝓣 ⊨.{u} p ↔ ∀ (𝓜 : Model.{u} 𝓣), 𝓜 ⊨ₛ p := by
   constructor
   · intro h 𝓜; apply h; exact 𝓜.satisfy_theory
   · intro h 𝓜 ρ h₁; rw [Vec.eq_nil ρ] at *; exact h ⟨𝓜, h₁⟩
 
-theorem satisfiable_iff {𝓣 : 𝓛.Theory} : Satisfiable.{u} 𝓣 ↔ Nonempty (Model.{u} 𝓣) := by
+theorem satisfiable_iff : Satisfiable.{u} 𝓣 ↔ Nonempty (Model.{u} 𝓣) := by
   constructor
   · intro ⟨𝓜, ρ, h⟩; rw [Vec.eq_nil ρ] at h; exact ⟨⟨𝓜, h⟩⟩
   · intro ⟨𝓜⟩; exists 𝓜, []ᵥ; apply 𝓜.satisfy_theory
 
-def Model.weaken {𝓣₁ 𝓣₂ : 𝓛.Theory} (𝓜 : 𝓣₁.Model) (h : 𝓣₂ ⊆ 𝓣₁) : 𝓣₂.Model where
-  toStructure := 𝓜.toStructure
-  satisfy_theory p h' := 𝓜.satisfy_theory p (h h')
-
 end Theory
 
-def Satisfiable.of_model {𝓣 : 𝓛.Theory} (𝓜 : Theory.Model.{u} 𝓣) : Satisfiable.{u} 𝓣 :=
-  Theory.satisfiable_iff.mpr ⟨𝓜⟩
+def Satisfiable.of_model {𝓣 : 𝓛.Theory} (𝓜 : Type u) [𝓛.IsStructure 𝓜] [𝓣.IsModel 𝓜] : Satisfiable.{u} 𝓣 :=
+  Theory.satisfiable_iff.mpr ⟨.of 𝓜⟩
 
-namespace Structure
+def theory (𝓜 : Type u) [𝓛.IsStructure 𝓜] : 𝓛.Theory := { p | 𝓜 ⊨ₛ p }
 
-def theory (𝓜 : 𝓛.Structure) : 𝓛.Theory := { p | 𝓜 ⊨ₛ p }
+instance : (𝓛.theory 𝓜).IsModel 𝓜 where
+  satisfy_theory _ h := h
 
-theorem theory.satisfiable {𝓜 : Structure.{u} 𝓛} : Satisfiable.{u} 𝓜.theory := by
-  rw [Theory.satisfiable_iff]; exact ⟨𝓜, λ _ h => h⟩
-
-end Structure
+theorem theory.satisfiable : Satisfiable.{u} (𝓛.theory 𝓜) := .of_model 𝓜
 
 
 
@@ -161,12 +176,12 @@ def ulift (𝓜 : Structure.{u} 𝓛) : Structure.{max u v} 𝓛 where
   interpFunc f v := ULift.up (𝓜.interpFunc f (ULift.down ∘ v))
   interpRel r v := 𝓜.interpRel r (ULift.down ∘ v)
 
-lemma interp_ulift {𝓜 : 𝓛.Structure} {ρ : 𝓜.Assignment n} :
+lemma interp_ulift {𝓜 : 𝓛.Structure} {ρ : Vec 𝓜 n} :
   ⟦ t ⟧ₜ 𝓜.ulift, (ULift.up ∘ ρ) = ULift.up (⟦ t ⟧ₜ 𝓜, ρ) := by
   induction t with simp
   | func f v ih => simp [ih]; rfl
 
-lemma satisfy_ulift {𝓜 : 𝓛.Structure} {ρ : 𝓜.Assignment n} :
+lemma satisfy_ulift {𝓜 : 𝓛.Structure} {ρ : Vec 𝓜 n} :
   𝓜.ulift ⊨[ULift.up ∘ ρ] p ↔ 𝓜 ⊨[ρ] p := by
   induction p with simp
   | rel r v => simp [interp_ulift]; rfl
@@ -195,16 +210,18 @@ theorem Satisfiable.up : Satisfiable.{u} Γ → Satisfiable.{max u v} Γ := by
 
 namespace Structure
 
+variable {𝓜 𝓝 : 𝓛.Structure}
+
 def ElementaryEquivalent (𝓜 : 𝓛.Structure) (𝓝 : 𝓛.Structure) :=
-  ∀ p, 𝓜 ⊨ₛ p ↔ 𝓝 ⊨ₛ p
+  ∀ (p : 𝓛.Sentence), 𝓜 ⊨ₛ p ↔ 𝓝 ⊨ₛ p
 infixr:25 " ≃ᴱ " => ElementaryEquivalent
 
-theorem ElementaryEquivalent.iff_theory_eq : 𝓜 ≃ᴱ 𝓝 ↔ 𝓜.theory = 𝓝.theory := by
+theorem ElementaryEquivalent.iff_theory_eq : 𝓜 ≃ᴱ 𝓝 ↔ 𝓛.theory 𝓜 = 𝓛.theory 𝓝 := by
   simp [ElementaryEquivalent, Set.ext_iff, theory]
 
 structure Embedding (𝓜 : 𝓛.Structure) (𝓝 : 𝓛.Structure) extends 𝓜 ↪ 𝓝 where
-  on_func : ∀ (f : 𝓛.Func n) (v : Vec 𝓜 n), toEmbedding (𝓜.interpFunc f v) = 𝓝.interpFunc f (toEmbedding ∘ v)
-  on_rel : ∀ (r : 𝓛.Rel n) (v : Vec 𝓜 n), 𝓜.interpRel r v ↔ 𝓝.interpRel r (toEmbedding ∘ v)
+  on_func {n} : ∀ (f : 𝓛.Func n) (v : Vec 𝓜 n), toEmbedding (IsStructure.interpFunc f v) = IsStructure.interpFunc f (toEmbedding ∘ v)
+  on_rel {n} : ∀ (r : 𝓛.Rel n) (v : Vec 𝓜 n), IsStructure.interpRel r v ↔ IsStructure.interpRel r (toEmbedding ∘ v)
 infixr:25 " ↪ᴹ " => Embedding
 
 namespace Embedding
@@ -221,16 +238,16 @@ def trans (e₁ : 𝓜 ↪ᴹ 𝓝) (e₂ : 𝓝 ↪ᴹ 𝓢) : 𝓜 ↪ᴹ 𝓢
   on_func f v := by simp [e₁.on_func, e₂.on_func]; rfl
   on_rel r v := by rw [e₁.on_rel, e₂.on_rel]; rfl
 
-theorem on_term (e : 𝓜 ↪ᴹ 𝓝) (t : 𝓛.Term n) (ρ : 𝓜.Assignment n) : e (⟦t⟧ₜ 𝓜, ρ) = ⟦t⟧ₜ 𝓝, e ∘ ρ := by
+theorem on_term (e : 𝓜 ↪ᴹ 𝓝) (t : 𝓛.Term n) (ρ : Vec 𝓜 n) : e (⟦t⟧ₜ 𝓜, ρ) = ⟦t⟧ₜ 𝓝, e ∘ ρ := by
   induction t with simp
   | func f v ih => rw [e.on_func]; congr; ext; simp [ih]
 
 def IsElementary (e : 𝓜 ↪ᴹ 𝓝) :=
-  ∀ {n} (p : 𝓛.Formula n) (ρ : 𝓜.Assignment n), 𝓜 ⊨[ρ] p ↔ 𝓝 ⊨[e ∘ ρ] p
+  ∀ {n} (p : 𝓛.Formula n) (ρ : Vec 𝓜 n), 𝓜 ⊨[ρ] p ↔ 𝓝 ⊨[e ∘ ρ] p
 
 /-- Tarski–Vaught test -/
 theorem is_elementary_iff (e : 𝓜 ↪ᴹ 𝓝) :
-  e.IsElementary ↔ ∀ {n} (p : 𝓛.Formula (n + 1)) (ρ : 𝓜.Assignment n), 𝓝 ⊨[e ∘ ρ] ∃' p → ∃ u, 𝓝 ⊨[e u ∷ᵥ e ∘ ρ] p := by
+  e.IsElementary ↔ ∀ {n} (p : 𝓛.Formula (n + 1)) (ρ : Vec 𝓜 n), 𝓝 ⊨[e ∘ ρ] ∃' p → ∃ u, 𝓝 ⊨[e u ∷ᵥ e ∘ ρ] p := by
   constructor
   · intro h n p ρ h₁
     rw [←h] at h₁; simp at h₁
@@ -259,8 +276,8 @@ theorem is_elementary_iff (e : 𝓜 ↪ᴹ 𝓝) :
 end Embedding
 
 structure Isomorphism (𝓜 : 𝓛.Structure) (𝓝 : 𝓛.Structure) extends 𝓜 ≃ 𝓝 where
-  on_func : ∀ (f : 𝓛.Func n) (v : Vec 𝓜 n), toEquiv (𝓜.interpFunc f v) = 𝓝.interpFunc f (toEquiv ∘ v)
-  on_rel : ∀ (r : 𝓛.Rel n) (v : Vec 𝓜 n), 𝓜.interpRel r v ↔ 𝓝.interpRel r (toEquiv ∘ v)
+  on_func {n} : ∀ (f : 𝓛.Func n) (v : Vec 𝓜 n), toEquiv (IsStructure.interpFunc f v) = IsStructure.interpFunc f (toEquiv ∘ v)
+  on_rel {n} : ∀ (r : 𝓛.Rel n) (v : Vec 𝓜 n), IsStructure.interpRel r v ↔ IsStructure.interpRel r (toEquiv ∘ v)
 infix:25 " ≃ᴹ " => Isomorphism
 
 namespace Isomorphism
@@ -287,11 +304,11 @@ def toEmbedding (i : 𝓜 ≃ᴹ 𝓝) : 𝓜 ↪ᴹ 𝓝 where
   on_func := i.on_func
   on_rel := i.on_rel
 
-theorem on_term (i : 𝓜 ≃ᴹ 𝓝) (t : 𝓛.Term n) (ρ : 𝓜.Assignment n) : i (⟦t⟧ₜ 𝓜, ρ) = ⟦t⟧ₜ 𝓝, i ∘ ρ := by
+theorem on_term (i : 𝓜 ≃ᴹ 𝓝) (t : 𝓛.Term n) (ρ : Vec 𝓜 n) : i (⟦t⟧ₜ 𝓜, ρ) = ⟦t⟧ₜ 𝓝, i ∘ ρ := by
   induction t with simp
   | func f v ih => rw [i.on_func]; congr; ext; simp [ih]
 
-theorem on_formula (i : 𝓜 ≃ᴹ 𝓝) (p : 𝓛.Formula n) (ρ : 𝓜.Assignment n) : 𝓜 ⊨[ρ] p ↔ 𝓝 ⊨[i ∘ ρ] p := by
+theorem on_formula (i : 𝓜 ≃ᴹ 𝓝) (p : 𝓛.Formula n) (ρ : Vec 𝓜 n) : 𝓜 ⊨[ρ] p ↔ 𝓝 ⊨[i ∘ ρ] p := by
   induction p with simp
   | rel r v => rw [i.on_rel]; congr!; simp [i.on_term]
   | eq t₁ t₂ => simp [←i.on_term]
